common/SmallstepLinking_.v
@@ -3,7 +3,6 @@ Require Import List.
 Require Import Events.
 Require Import Globalenvs.
 Require Import LanguageInterface_.
-Require Import Smallstep.
 Require Import Smallstep_.
 Require Import Linking.
 Require Import Classical.
@@ -22,8 +21,7 @@ Ltac subst_dep :=
   end.
 
 Section LINK.
-  Context {li} (L: bool -> semantics li li).
-  Let I := bool.
+  Context {I li} (L: I -> semantics li li).
 
   (** * Definition *)
 
@@ -73,7 +71,7 @@ Section LINK.
 
   Context (sk: AST.program unit unit).
 
-  Program Definition semantics: semantics li li :=
+  Program Definition semantics': semantics li li :=
     {|
       activate se :=
         {|
@@ -85,7 +83,7 @@ Section LINK.
           globalenv := tt;
         |};
       skel := sk;
-      footprint i := footprint (L true) i \/ footprint (L false) i;
+      footprint x := exists i, footprint (L i) x;
     |}.
   Next Obligation.
     inv H0.
@@ -115,8 +113,7 @@ Section LINK.
   (** * Receptiveness and determinacy *)
 
   (* Lemma semantics_receptive: *)
-  (*   (forall i, receptive (L i)) -> *)
-  (*   receptive semantics. *)
+  (*   (forall i, receptive (L i)) -> receptive semantics'. *)
   (* Proof. *)
   (*   intros HL se. unfold receptive in HL. *)
   (*   constructor; cbn. *)
@@ -184,9 +181,8 @@ End LINK.
 (** ** Simulation relation *)
 
 Section FSIM.
+  Context {I: Type}.
   Context {li1 li2} (cc: callconv li1 li2).
-
-  Notation I := bool.
   Context (L1 : I -> Smallstep_.semantics li1 li1).
   Context (L2 : I -> Smallstep_.semantics li2 li2).
   Context (HL : forall i, fsim_components cc cc (L1 i) (L2 i)).
@@ -324,8 +320,8 @@ Section FSIM.
 
   Lemma semantics_simulation sk1 sk2:
     fsim_properties cc cc se1 se2 w pset
-      (semantics L1 sk1 se1)
-      (semantics L2 sk2 se2)
+      (semantics' L1 sk1 se1)
+      (semantics' L2 sk2 se2)
       index order match_states.
   Proof.
     split; cbn.
@@ -342,6 +338,8 @@ End FSIM.
 (** * Linking operator *)
 
 Local Unset Program Cases.
+
+Definition semantics {li} := @semantics' bool li.
 
 Definition compose {li} (La Lb: Smallstep_.semantics li li) :=
   let L i := match i with true => La | false => Lb end in
@@ -364,7 +362,7 @@ Proof.
   eapply Forward_simulation with (order cc L1 L2 HL) (match_states cc L1 L2 HL).
   - destruct Ha, Hb. cbn. congruence.
   - intros i. cbn. destruct Ha, Hb.
-    rewrite fsim_footprint, fsim_footprint0. reflexivity.
+    split; (intros [[|] Hix]; [exists true | exists false]); cbn in *; firstorder.
   - intros se1 se2 w qset Hse Hse1.
     eapply semantics_simulation; eauto.
     pose proof (link_linkorder _ _ _ Hsk1) as [Hsk1a Hsk1b].
@@ -373,3 +371,337 @@ Proof.
     induction (fsim_order_wf (HL i) x) as [x Hx IHx].
     constructor. intros z Hxz. inv Hxz; subst_dep. eauto.
 Qed.
+
+Section LEVEL.
+
+  Context {I: Type} {J: I -> Type}.
+  Context {li} (L: forall i, J i -> Smallstep_.semantics li li).
+
+  Variable (sk: AST.program unit unit).
+
+  Let S1' i := (fun j => L i j).
+  Let S1 := (fun i => semantics' (S1' i) sk).
+  Let S2 := (fun p => L (projT1 p) (projT2 p)).
+
+  Let L1 := semantics' S1 sk.
+  Let L2 := semantics' S2 sk.
+
+  Inductive match_levels: state L1 -> state L2 -> Prop :=
+  | match_nil: match_levels nil nil
+  | match_i i j s k1 k2:
+      match_levels k1 k2 ->
+      match_levels (st S1 i (st (S1' i) j s :: nil) :: k1) (st S2 (existT _ i j) s :: k2)
+  | match_j i j s k ks k1 k2:
+      match_levels (st S1 i (k :: ks) :: k1) k2 ->
+      match_levels (st S1 i (st (S1' i) j s :: k :: ks) :: k1)
+                   (st S2 (existT _ i j) s :: k2).
+  Hint Constructors match_levels.
+  Hint Constructors initial_state final_state at_external after_external.
+
+  Lemma level_simulation1: forward_simulation 1 1 L1 L2.
+  Proof.
+    constructor. econstructor. reflexivity.
+    - intros x. cbn. split.
+      + intros [i [j H]]. exists (existT _ i j). apply H.
+      + intros [ij H]. exists (projT1 ij), (projT2 ij). apply H.
+    - intros se ? [ ] qset [ ] Hse.
+      instantiate (1 := fun _ _ _ => _). cbn beta.
+      eapply forward_simulation_step
+        with (match_states := match_levels).
+      + intros q ? s1 [ ] H. inv H. inv H1. cbn in *.
+        exists (st S2 (existT _ i i0) s0 :: nil). split; auto.
+      + intros s1 s2 r Hs Hr. inv Hr. inv H.
+        inv Hs. subst_dep. inv H5.
+        exists r. split; constructor; auto.
+      + intros s1 s2 q Hs Hq. inv Hq. inv H.
+        inv Hs; subst_dep.
+        * exists tt, q. repeat apply conj; try constructor; auto.
+          -- intros [ix jx]. unfold S1', S1, S2 in *; cbn in *.
+             specialize (H0 ix). intros Hx. apply H0. firstorder.
+          -- intros r ? s1' [ ] Hr. inv Hr. inv H7.
+             subst_dep. inv H4. subst_dep.
+             eexists. split; constructor; eauto.
+        * exists tt, q. repeat apply conj; try constructor; auto.
+          -- intros [ix jx]. unfold S1', S1, S2 in *; cbn in *.
+             specialize (H0 ix). intros Hx. apply H0. firstorder.
+          -- intros r ? s1' [ ] Hr. inv Hr. inv H7.
+             subst_dep. inv H4. subst_dep.
+             eexists. split; constructor; eauto.
+      + intros s1 t s1' Hstep s2 Hs. inv Hstep.
+        (* Internal step of L i *)
+        * inv H.
+          (* Internal step of L i j *)
+          -- inv Hs; subst_dep; eexists.
+             ++ split; [ apply step_internal | econstructor ]; eauto.
+             ++ split; [ apply step_internal | econstructor ]; eauto.
+          (* L i j calls into L i j' *)
+          -- inv Hs; subst_dep; eexists.
+             ++ split; [ eapply step_push | ]; eauto; auto.
+             ++ split; [ eapply step_push | ]; eauto; auto.
+          (* L i j returns to L i j' *)
+          -- inv Hs. subst_dep. inv H8; subst_dep; eexists.
+             ++ split; [ eapply step_pop | ]; eauto.
+             ++ split; [ eapply step_pop | ]; eauto.
+        (* L i j calls into L i' j' *)
+        * inv H. inv H1. inv Hs; subst_dep; eexists.
+          -- split; [ eapply step_push | ]; eauto; auto.
+          -- split; [ eapply step_push | ]; eauto; auto.
+        (* L i j return to L i' j' *)
+        * inv H. inv H0. inv Hs; subst_dep. inv H6; subst_dep; eexists.
+          -- split; [ eapply step_pop | ]; eauto.
+          -- split; [ eapply step_pop | ]; eauto.
+    - apply well_founded_ltof.
+  Qed.
+
+  Lemma foo: forall i j s t, st S2 (existT J i j) s = st S2 (existT J i j) t -> s = t.
+  Proof.
+    intros. inv H. subst_dep. auto.
+  Qed.
+
+  Hypothesis I_dec: forall (ix iy: I), {ix = iy} + {ix <> iy}.
+
+  Hypothesis valid_query_excl:
+    forall i i' j j' se q,
+      valid_query (li := li) (L i j) se q -> valid_query (L i' j') se q ->
+      existT _ i j = existT _ i' j'.
+
+  (* FIXME: clean up the proof *)
+  Lemma level_simulation2: forward_simulation 1 1 L2 L1.
+  Proof.
+    constructor. econstructor. reflexivity.
+    - intros x. cbn. split.
+      + intros [ij H]. exists (projT1 ij), (projT2 ij). apply H.
+      + intros [i [j H]]. exists (existT _ i j). apply H.
+    - intros se ? [ ] qset [ ] Hse.
+      instantiate (1 := fun _ _ _ => _). cbn beta.
+      eapply forward_simulation_step
+        with (match_states := fun s1 s2 => match_levels s2 s1).
+      + intros q ? s1 [ ] H. inv H.
+        destruct i as [i j]. eexists. split.
+        * constructor. instantiate (1 := i). firstorder.
+          constructor. instantiate (1 := j). firstorder.
+          eauto.
+        * auto.
+      + intros s1 s2 r Hs Hr. inv Hr.
+        remember (st S2 i s :: nil) as xs. inv Hs.
+        * inv H1.
+        * remember (st S2 (existT J i0 j) s0) as x.
+          remember (st S2 i s) as y. inv H2.
+          inversion H3. subst. apply foo in H3. subst.
+          eexists. split; [ | constructor ].
+          inv H0. constructor. constructor. auto.
+        * inv H2. inv H0.
+      + intros s1 s2 q Hs H. inv H.
+        remember (st S2 i s :: k) as xs. inversion Hs.
+        * subst. inv H2.
+        * subst. remember (st S2 (existT J i0 j) s0) as x.
+          remember (st S2 i s) as y. inv H3.
+          inversion H4. subst. apply foo in H4. subst.
+          exists tt, q. repeat apply conj; try constructor.
+          -- constructor. auto. intros j0.
+             specialize (H1 (existT _ i0 j0)). firstorder.
+          -- intros ix. intros Hx. firstorder.
+             specialize (H1 (existT _ ix x0)).
+             apply H1. firstorder.
+          -- intros r ? s1' [ ] Hr. inv Hr.
+             subst_dep. eexists; split.
+             ++ constructor. constructor. eauto.
+             ++ constructor. auto.
+        * subst. remember (st S2 (existT J i0 j) s0) as x.
+          remember (st S2 i s) as y. inv H3.
+          inversion H4. subst. apply foo in H4. subst.
+          exists tt, q. repeat apply conj; try constructor.
+          -- constructor. auto. intros j0.
+             specialize (H1 (existT _ i0 j0)). firstorder.
+          -- intros ix. intros Hx. firstorder.
+             specialize (H1 (existT _ ix x0)).
+             apply H1. firstorder.
+          -- intros r ? s1' [ ] Hr. inv Hr.
+             subst_dep. eexists; split.
+             ++ constructor. constructor. eauto.
+             ++ constructor. auto.
+      + intros s1 t s1' Hstep s2 Hs. inv Hstep.
+        (* internal step *)
+        * remember (st S2 i s :: k) as xs. inversion Hs.
+          -- subst. inv H1.
+          -- subst. remember (st S2 (existT J i0 j) s0) as x.
+             remember (st S2 i s) as y. inv H2.
+             inversion H3. subst. apply foo in H3. subst.
+             eexists. split.
+             ++ apply step_internal. apply step_internal. eauto.
+             ++ constructor. auto.
+          -- subst. remember (st S2 (existT J i0 j) s0) as x.
+             remember (st S2 i s) as y. inv H2.
+             inversion H3. subst. apply foo in H3. subst.
+             eexists. split.
+             ++ apply step_internal. apply step_internal. eauto.
+             ++ constructor. auto.
+        (* function call *)
+        * remember (st S2 i s :: k) as xs. inversion Hs.
+          -- subst. inv H3.
+          -- subst. remember (st S2 (existT J i0 j0) s0) as x.
+             remember (st S2 i s) as y. inv H4.
+             inversion H5. subst. apply foo in H5. subst.
+             destruct j as [i j]. destruct (I_dec i i0).
+             ++ subst. eexists. split.
+                apply step_internal. eapply step_push; eauto. auto.
+             ++ eexists. split.
+                eapply step_push. econstructor. apply H.
+                intros j1 Hx. apply n.
+                exploit valid_query_excl. apply H0. apply Hx.
+                apply eq_sigT_fst.
+                instantiate (1 := i). firstorder.
+                constructor. apply H0. eauto. auto.
+          -- subst. remember (st S2 (existT J i0 j0) s0) as x.
+             remember (st S2 i s) as y. inv H4.
+             inversion H5. subst. apply foo in H5. subst.
+             destruct j as [i j]. destruct (I_dec i i0).
+             ++ subst. eexists. split.
+                apply step_internal. eapply step_push; eauto. auto.
+             ++ eexists. split.
+                eapply step_push. econstructor. apply H.
+                intros j1 Hx. apply n.
+                exploit valid_query_excl. apply H0. apply Hx.
+                apply eq_sigT_fst.
+                instantiate (1 := i). firstorder.
+                constructor. apply H0. eauto. auto.
+        (* function return *)
+        * remember (st S2 i s :: st S2 j sk0 :: k) as xs.
+          inversion Hs; subst.
+          -- inv H2.
+          -- remember (st S2 (existT J i0 j0) s0) as x.
+             remember (st S2 i s) as y. inv H3.
+             inversion H4. subst. apply foo in H4. subst.
+
+             remember (st S2 j sk0) as xs. inversion H1; subst.
+             ++ inversion H2. subst. apply foo in H2. subst.
+                eexists. split.
+                eapply step_pop. constructor. eauto.
+                constructor. eauto. auto.
+             ++ inversion H2. subst. apply foo in H2. subst.
+                eexists. split.
+                eapply step_pop. constructor. eauto.
+                constructor. eauto. auto.
+          -- remember (st S2 (existT J i0 j0) s0) as x.
+             remember (st S2 i s) as y. inv H3.
+             inversion H4. subst. apply foo in H4. subst.
+
+             remember (st S2 j sk0) as xs. inv H1.
+             ++ inversion H7. subst. apply foo in H7.
+                subst_dep. eexists. split.
+                eapply step_internal. eapply step_pop.
+                eauto. eauto. auto.
+             ++ inversion H7. subst. apply foo in H7.
+                subst_dep. eexists. split.
+                eapply step_internal. eapply step_pop.
+                eauto. eauto. auto.
+    - apply well_founded_ltof.
+  Qed.
+
+End LEVEL.
+
+Require Import Coq.Logic.FinFun.
+
+Lemma bij_surj {A B} (f: A -> B): Bijective f -> Surjective f.
+Proof.
+  intros [g [H1 H2]] b. exists (g b). easy.
+Qed.
+
+Lemma bij_inj {A B} (f: A -> B): Bijective f -> Injective f.
+Proof.
+  intros [g [H1 H2]] x y H.
+  rewrite <- (H1 x).
+  rewrite <- (H1 y). congruence.
+Qed.
+
+Section MAP.
+
+  Context {I li} (L: I -> Smallstep_.semantics li li).
+  Context {J} {F: J -> I} (HF: Bijective F).
+  Variable (sk: AST.program unit unit).
+
+  Let LF := semantics' (fun i => L (F i)) sk.
+
+  Inductive match_bijection: state (semantics' L sk) -> state LF -> Prop :=
+  | match_bijection_cons i j s s' k k':
+      @existT I (fun i => state (L i)) i s = @existT I (fun i => state (L i)) (F j) s' ->
+      match_bijection k k' ->
+      match_bijection (st L i s :: k) (st (fun i => L (F i)) j s'  :: k')
+  | match_bijection_nils: match_bijection nil nil.
+
+  Hint Constructors match_bijection.
+
+  Definition switch_index {i j} (H: i = F j) (s: state (L i)): state (L (F j)).
+  Proof.
+    rewrite <- H. exact s.
+  Defined.
+
+  Lemma bijective_map_simulation1: forward_simulation 1 1 (semantics' L sk) LF.
+  Proof.
+    constructor. econstructor. reflexivity.
+    - intros id. split; intros [i Hi].
+      + apply bij_surj in HF.
+        specialize (HF i) as [x Hx].
+        exists x. congruence.
+      + exists (F i). auto.
+    - intros se ? [ ] qset [ ] Hse.
+      instantiate (1 := fun _ _ _ => _). cbn beta.
+      apply bij_surj in HF.
+      eapply forward_simulation_step with (match_states := match_bijection).
+      + intros q ? s [ ] H. inv H.
+        specialize (HF i) as [j Hj]. subst.
+        eexists; split; constructor; eauto.
+      + intros s1 s2 r Hs H. inv H. inv Hs. inv H5.
+        inv H4. subst_dep. exists r. split; constructor; auto.
+      + intros s1 s2 q Hs H. inv H. inv Hs. inv H5.
+        subst_dep. exists tt, q. repeat apply conj; try constructor; auto.
+        intros r ? s1' [ ] H. inv H. subst_dep.
+        eexists. split; constructor; eauto.
+      + intros s1 t s1' Hstep s2 Hs. inv Hstep; inv Hs.
+        * inv H4. subst_dep. eexists; split.
+          eapply step_internal; eauto.
+          constructor; eauto.
+        * specialize (HF j) as [x Hx]. subst.
+          inv H6. subst_dep. eexists. split.
+          eapply step_push; eauto. auto.
+        * inv H5. subst_dep. inv H6. inv H5. subst_dep.
+          eexists. split. eapply step_pop; eauto. auto.
+    - apply well_founded_ltof.
+  Qed.
+
+  Lemma bijective_map_simulation2: forward_simulation 1 1 LF (semantics' L sk).
+  Proof.
+    constructor. econstructor. reflexivity.
+    - intros id. split; intros [i Hi].
+      + exists (F i). auto.
+      + apply bij_surj in HF.
+        specialize (HF i) as [x Hx].
+        exists x. congruence.
+    - intros se ? [ ] qset [ ] Hse.
+      instantiate (1 := fun _ _ _ => _). cbn beta.
+      eapply forward_simulation_step
+        with (match_states := fun s1 s2 => match_bijection s2 s1).
+      + intros q ? s [ ] H. inv H.
+        eexists; split; constructor; eauto.
+      + intros s1 s2 r Hs H. inv H. inv Hs.
+        inv H3. subst_dep. inv H5.
+        eexists; split; constructor; auto.
+      + intros s1 s2 q Hs H. inv H.
+        inv Hs. inv H4. subst_dep.
+        exists tt, q. repeat apply conj; try constructor; auto.
+        * intros j. apply bij_surj in HF.
+          specialize (HF j) as [x <-]. easy.
+        * intros r ? s1' [ ] H. inv H. subst_dep.
+          eexists; split; constructor; auto. auto.
+      + intros s1 t s1' Hstep s2 Hs. inv Hstep; inv Hs.
+        * inv H3. subst_dep. eexists; split.
+          apply step_internal; eauto. auto.
+        * inv H5. subst_dep. eexists; split.
+          eapply step_push; eauto. auto.
+        * inv H4. subst_dep. inv H6. inv H4. subst_dep.
+          eexists; split.
+          eapply step_pop; eauto. auto.
+    - apply well_founded_ltof.
+  Qed.
+
+End MAP.
